\documentclass[12pt]{article}
\usepackage{amsmath}
\begin{document}
	\begin{align*}
		a^2 &= \dfrac{\partial P}{\partial \rho} + \dfrac{p}{\rho ^2}\dfrac{\partial P}{\partial e} \\
		&=(\gamma -1)e + \dfrac{P}{\rho}(\gamma -1)
	\end{align*}
	
	Recall:
	
	\begin{equation}
		P = (\gamma -1) \rho e - \gamma P^{\infty}
	\end{equation}
	
	We get: 
	
	\begin{align*}
		(\gamma -1)\rho e = P+\gamma p^{\infty}
	\end{align*}
	
	Then, multiply both sides by $\rho$
	
	\begin{align*}
		a^2 \rho &= (\gamma -1)\rho e + P(\gamma -1)\\
		a^2 \rho &= (P+ \gamma P^{\infty})+P(\gamma-1)\\
		a^2&=\dfrac{\gamma (P+P^{\infty}) }{\rho} \\
		a&=\sqrt{\dfrac{\gamma (P+P^{\infty}) }{\rho}}
	\end{align*}
	
	 
\end{document}